# Composite Functions

To help you master finding the general expression for composite functions, here are three problems that require you to substitute the entire function $f(x)$ into $g(x)$.

This process is like a "nested" substitution: everywhere you see an $x$ in the outer function, you replace it with the entire formula of the inner function.

------

## Practice Problems (Algebraic Expressions)

### Problem 1

Given $f(x) = 3x - 1$ and $g(x) = \frac{x^2}{x + 5}$, find the expression for $g(f(x))$.

### Problem 2

Given $f(x) = x + 4$ and $g(x) = \frac{x^2 - 16}{x - 2}$, find the expression for $g(f(x))$ and simplify.

### Problem 3

Given $f(x) = 2x^2$ and $g(x) = \frac{x - 3}{x + 1}$, find the expression for $g(f(x))$.

------

## Answer Key and Step-by-Step Solutions

### Solution 1:

1. Substitute $f(x)$ into $g(x)$: Replace every $x$ in $g(x)$ with $(3x - 1)$.

   

   $$g(f(x)) = \frac{(3x - 1)^2}{(3x - 1) + 5}$$

2. **Simplify:**

   - Numerator: $(3x - 1)(3x - 1) = 9x^2 - 6x + 1$
   - Denominator: $3x - 1 + 5 = 3x + 4$

- **Answer:** $\frac{9x^2 - 6x + 1}{3x + 4}$

### Solution 2:

1. Substitute $f(x)$ into $g(x)$: Replace every $x$ in $g(x)$ with $(x + 4)$.

   

   $$g(f(x)) = \frac{(x + 4)^2 - 16}{(x + 4) - 2}$$

2. **Simplify:**

   - Numerator: $(x^2 + 8x + 16) - 16 = x^2 + 8x$
   - Denominator: $x + 4 - 2 = x + 2$

- **Answer:** $\frac{x^2 + 8x}{x + 2}$ (or $\frac{x(x + 8)}{x + 2}$)

### Solution 3:

1. Substitute $f(x)$ into $g(x)$: Replace every $x$ in $g(x)$ with $(2x^2)$.

   

   $$g(f(x)) = \frac{(2x^2) - 3}{(2x^2) + 1}$$

- **Answer:** $\frac{2x^2 - 3}{2x^2 + 1}$

